src/tls/MasterSecret.fst
@@ -1,6 +1,7 @@
 (* An experiment towards the PRF in KeySchedule, collapsing master and key derivation *)
 module MasterSecret (* : ST _ _ _ *)
 open FStar.HyperHeap
+open FStar.HyperStack
 open TLSConstants
 open StreamAE
 open TLSInfo
