src/tls/StreamPlain.fst
@@ -57,7 +57,7 @@ let repr i len f =
   let payload = Content.repr i f in 
   pad payload ct len
 
-private inline let min (a:nat) (b:nat): nat = if a < b then a else b
+private unfold let min (a:nat) (b:nat): nat = if a < b then a else b
 
 // Implementations MUST NOT send zero-length fragments of Handshake,
 // Alert, or ChangeCipherSpec content types. Zero-length fragments of
